internal/examples/semantics/INTERFACES.md
@@ -2,8 +2,8 @@
 
 ### Basic Interfaces
 [X] Create tuple of methods, ie `(catHello, catBye)`
-[X] Return (method, typeDescriptor, value) when interface is called, value is a pointer to original value 
-[X] Create interfaceT type in coq, defined by a list of arrowT methods, including `interfaceT []` empty interface 
+[-] Return (method, typeDescriptor, value) when interface is called, value is a pointer to original value 
+[-] Create interfaceT type in coq, defined by a list of arrowT methods, including `interfaceT []` empty interface 
 [X] No proofs for now, including typecheck
 
 ### Type Switches 
@@ -15,7 +15,7 @@ func switch(x interface{}) ...
 
 [X] Built method table as collection of methods, string, anyT (needs dynamic value)
 [] Sort order of methods
-[X] Use struct for collection of methods (use search field by name function), ie
+[-] Use struct for collection of methods (use search field by name function), ie
 
 ```
 (getMethod x.1 "Get" )
